Weights for LATE conditional on covariates

July 12, 2022

Deriving weights

Suppose there are covariates (X, V). For simplicity, suppose X and V are discrete. The LATE for $z_0 \rightarrow z_1$ conditional on V = v is

By Bayes' rule, $\mathbb{P}\{X = x \mid \text{Complier}, V = v\}$ can be written as

$$\mathbb{P}\{X = x \mid \text{Complier}, V = v\} = \frac{\mathbb{P}\{\text{Complier} \mid V = v, X = x\} \times \mathbb{P}\{X = x \mid V = v\}}{\mathbb{P}\{\text{Complier} \mid V = v\}} \\ = \frac{[p(x, v, z_1) - p(x, v, z_0)] \times \mathbb{P}\{X = x \mid V = v\}}{\sum_{x' \in \text{supp}(X)} [p(x', v, z_1) - p(x', v, z_0)] \times \mathbb{P}\{X = x' \mid V = v\}}.$$
(2)

By substituting (2) into (1), we have

$$\begin{split} \mathbb{E}[LATE(X,V) \mid \text{Complier}, V = v] \\ &= \sum_{x \in \text{supp}(X)} \int_{p(x,v,z_0)}^{p(x,v,z_1)} \left[m(1 \mid u, x, v) - m(0 \mid u, x, v) \right] \frac{1}{p(x,v,z_1) - p(x,v,z_0)} \, du \\ &\qquad \times \frac{\left[p(x,v,z_1) - p(x,v,z_0) \right] \times \mathbb{P}\{X = x \mid V = v\}}{\sum_{x' \in \text{supp}(X)} \left[p(x',v,z_1) - p(x',v,z_0) \right] \times \mathbb{P}\{X = x' \mid V = v\}}. \\ &= \sum_{x \in \text{supp}(X)} \int_{p(x,v,z_0)}^{p(x,v,z_1)} \left[m(1 \mid u, x, v) - m(0 \mid u, x, v) \right] \, du \\ &\qquad \times \frac{\mathbb{P}\{X = x \mid V = v\}}{\sum_{x' \in \text{supp}(X)} \left[p(x',v,z_1) - p(x',v,z_0) \right] \times \mathbb{P}\{X = x' \mid V = v\}}. \end{split}$$

Implementing weights

The ivmte package already estimates

$$\int_{p(x,v,z_0)}^{p(x,v,z_1)} m(1 \mid u, x, v) - m(0 \mid u, x, v) \, du \tag{3}$$

for every observation in the data. Then averaging the estimates of (3) across the subset of observations with V = v provides an estimate of

$$\sum_{x \in \text{supp}(X)} \int_{p(x,v,z_0)}^{p(x,v,z_1)} \left[m(1 \mid u, x, v) - m(0 \mid u, x, v) \right] \, du \times \mathbb{P}\{X = x \mid V = v\}.$$
(4)

Then all that remains for estimating $\mathbb{E}[LATE(X, V) \mid ComplierV = v]$ is to divide (4) by an estimate of

$$\sum_{x \in \text{supp}(X)} \left[p(x, v, z_1) - p(x, v, z_0) \right] \times \mathbb{P}\{X = x \mid V = v\},\$$

which is straightforward to obtain.